Iris/Iris/HeapLang/Lib/Lock.lean
@@ -22,10 +22,8 @@ class lock (GF : BundledGFunctors) [IrisGS_gen hlc Exp GF] where
   is_lock : lockG GF → name → Val → IProp GF → IProp GF
   locked : lockG GF → name → IProp GF
 
-  is_lock_persistent {N} γ lk (R : IProp GF) :
-    Persistent (is_lock N γ lk R)
-  is_lock_iff {N} γ lk (R₁ R₂ : IProp GF) :
-    is_lock N γ lk R₁ ⊢ (▷ □ (R₁ ∗-∗ R₂)) -∗ is_lock N γ lk R₂
+  is_lock_persistent {N} γ lk (R : IProp GF) : Persistent (is_lock N γ lk R)
+  is_lock_iff {N} γ lk (R₁ R₂ : IProp GF) : is_lock N γ lk R₁ ⊢ (▷ □ (R₁ ∗-∗ R₂)) -∗ is_lock N γ lk R₂
 
   locked_timeless {N} γ : Timeless (locked N γ)
   locked_exclusive {N} γ : locked N γ ∗ locked N γ ⊢@{IProp GF} False
@@ -38,34 +36,33 @@ class lock (GF : BundledGFunctors) [IrisGS_gen hlc Exp GF] where
   acquire_spec {N} γ lk R :
     ⊢ □ ∀ (Φ : Val → IProp GF),
     is_lock N γ lk R
-    -∗ ((locked N γ ∗ R) -∗ Φ (.lit .unit))
+    -∗ ((locked N γ ∗ R) -∗ Φ hl_val(#()))
     -∗ WP hl({acquire} {lk}) {{ Φ }}
   release_spec {N} γ lk R :
     ⊢ □ ∀ (Φ : Val → IProp GF),
     (is_lock N γ lk R) ∗ locked N γ ∗ R
-    -∗ (True -∗ Φ (.lit .unit))
+    -∗ (True -∗ Φ hl_val(#()))
     -∗ WP hl({release} {lk}) {{ Φ }}
 
-instance lock_name_inhabited [IrisGS_gen hlc Exp GF] [lk : lock GF] : Inhabited lk.name := lk.lock_name_inhabited
+instance lock_name_inhabited [IrisGS_gen hlc Exp GF] [lk : lock GF] : Inhabited lk.name :=
+  lk.lock_name_inhabited
 
 section lemmas
 
 variable [IrisGS_gen hlc Exp GF] [lk : lock GF] (N : lk.lockG GF)
 
-instance is_lock_persistent_inst γ v R :
-    Persistent (lk.is_lock N γ v R) :=
+instance is_lock_persistent_inst γ v R : Persistent (lk.is_lock N γ v R) :=
   lk.is_lock_persistent γ v R
 
-instance locked_timeless_inst γ :
-    Timeless (lk.locked N γ) :=
+instance locked_timeless_inst γ : Timeless (lk.locked N γ) :=
   lk.locked_timeless γ
 
 theorem is_lock_contractive γ v :
     OFE.Contractive (lk.is_lock N γ v) := by
   rw [contractive_internalEq (PROP := IProp GF)]
   iintro %x₁ %x₂ #HEQ
-  iapply BI.prop_ext
-  iintro !>
+  iapply prop_ext
+  imodintro
   isplit
   · iintro #H
     iapply lock.is_lock_iff $$ H
@@ -80,8 +77,7 @@ theorem is_lock_contractive γ v :
     · exact ⟨fun _ _ _ h => wandIff_ne.ne .rfl h⟩
     · iapply equiv_wandIff; exact .rfl
 
-instance is_lock_ne γ v :
-    OFE.NonExpansive (lk.is_lock N γ v) :=
+instance is_lock_ne γ v : OFE.NonExpansive (lk.is_lock N γ v) :=
   letI := is_lock_contractive N γ v
   OFE.ne_of_contractive _
 
@@ -95,7 +91,6 @@ theorem newlock_spec R :
   iapply lk.newlock_spec_delay_init $$ %(fun v => iprop(|={⊤}=> Φ v))
   iintro %v %γ Hinit
   imod Hinit $$ %R %⊤ HR
-  imodintro
   iapply HΦ $$ Hinit
 
 end lemmas
